example/Dispatcher.thy
@@ -1,0 +1,167 @@
+theory Dispatcher
+
+imports
+  "../Parse"
+  "../attic/BasicBlocks"
+  "../Hoare/Hoare"
+
+begin
+
+definition 
+dispatch1_hash :: "256 word"
+where
+"dispatch1_hash == 0x3ecb5edf"
+
+definition 
+dispatch2_hash :: "256 word"
+where
+"dispatch2_hash == 0x8cd5b077"
+
+lemmas blocks_simps = build_blocks_def byteListInt_def find_block_def extract_indexes_def build_vertices_def
+ aux_basic_block.simps add_address_def block_pt_def
+
+
+
+value"blocks_list (build_blocks (parse_bytecode ''60606040526000357c0100000000000000000000000000000000000000000000000000000000900463ffffffff1680633ecb5edf1460475780638cd5b07714607b575b600080fd5b3415605157600080fd5b6065600480803590602001909190505060a1565b6040518082815260200191505060405180910390f35b3415608557600080fd5b608b60ad565b6040518082815260200191505060405180910390f35b6000600190505b919050565b6000600290505b905600a165627a7a72305820c9cf1e9d83721f6f9afecea62b7e868d98502ee8556dcaf6abb24acb8bc0d9fb0029''))"
+
+definition insts where
+"insts \<equiv>
+[Stack (PUSH_N [96]), Stack (PUSH_N [64]), Memory MSTORE, Stack (PUSH_N [0]), Stack CALLDATALOAD,
+  Stack (PUSH_N [1, 0, 0, 0, 0, 0, 0, 0, 0, 0, 0, 0, 0, 0, 0, 0, 0, 0, 0, 0, 0, 0, 0, 0, 0, 0, 0, 0, 0]),
+  Swap 1, Arith DIV, Stack (PUSH_N [255, 255, 255, 255]), Bits inst_AND, Dup 1,
+  Stack (PUSH_N [62, 203, 94, 223]), Arith inst_EQ, Stack (PUSH_N [71]), Pc JUMPI, Dup 1,
+  Stack (PUSH_N [140, 213, 176, 119]), Arith inst_EQ, Stack (PUSH_N [123]), Pc JUMPI, Pc JUMPDEST,
+  Stack (PUSH_N [0]), Dup 1, Unknown 253, Pc JUMPDEST, Info CALLVALUE, Arith ISZERO, Stack (PUSH_N [81]),
+  Pc JUMPI, Stack (PUSH_N [0]), Dup 1, Unknown 253, Pc JUMPDEST, Stack (PUSH_N [101]), Stack (PUSH_N [4]),
+  Dup 1, Dup 1, Stack CALLDATALOAD, Swap 1, Stack (PUSH_N [32]), Arith ADD, Swap 1, Swap 2, Swap 1, Stack POP,
+  Stack POP, Stack (PUSH_N [161]), Pc JUMP, Pc JUMPDEST, Stack (PUSH_N [64]), Memory MLOAD, Dup 1, Dup 3,
+  Dup 2, Memory MSTORE, Stack (PUSH_N [32]), Arith ADD, Swap 2, Stack POP, Stack POP, Stack (PUSH_N [64]),
+  Memory MLOAD, Dup 1, Swap 2, Arith SUB, Swap 1, Misc RETURN, Pc JUMPDEST, Info CALLVALUE, Arith ISZERO,
+  Stack (PUSH_N [133]), Pc JUMPI, Stack (PUSH_N [0]), Dup 1, Unknown 253, Pc JUMPDEST, Stack (PUSH_N [139]),
+  Stack (PUSH_N [173]), Pc JUMP, Pc JUMPDEST, Stack (PUSH_N [64]), Memory MLOAD, Dup 1, Dup 3, Dup 2,
+  Memory MSTORE, Stack (PUSH_N [32]), Arith ADD, Swap 2, Stack POP, Stack POP, Stack (PUSH_N [64]),
+  Memory MLOAD, Dup 1, Swap 2, Arith SUB, Swap 1, Misc RETURN, Pc JUMPDEST, Stack (PUSH_N [0]),
+  Stack (PUSH_N [1]), Swap 1, Stack POP, Pc JUMPDEST, Swap 2, Swap 1, Stack POP, Pc JUMP, Pc JUMPDEST,
+  Stack (PUSH_N [0]), Stack (PUSH_N [2]), Swap 1, Stack POP, Pc JUMPDEST, Swap 1, Pc JUMP, Misc STOP, Log LOG1,
+  Stack (PUSH_N [98, 122, 122, 114, 48, 88]), Arith SHA3, Unknown 201, Unknown 207, Unknown 30, Swap 14, Dup 4,
+  Stack (PUSH_N [31, 111, 154, 254, 206, 166, 43, 126, 134, 141, 152, 80, 46, 232, 85, 109, 202, 246, 171]),
+  Unknown 178, Unknown 74, Unknown 203, Dup 12, Unknown 192, Unknown 217, Unknown 251, Misc STOP, Unknown 41]"
+
+definition blocks where
+"blocks =
+\<lparr>blocks_indexes = [0, 56, 66, 71, 77, 81, 101, 123, 129, 133, 139, 161, 168, 173, 180, 183, 184, 226],
+    blocks_list = map_of [(0, [(0, Stack (PUSH_N [96])), (2, Stack (PUSH_N [64])), (4, Memory MSTORE), (5, Stack (PUSH_N [0])),
+            (7, Stack CALLDATALOAD),
+            (8, Stack (PUSH_N
+                        [1, 0, 0, 0, 0, 0, 0, 0, 0, 0, 0, 0, 0, 0, 0, 0, 0, 0, 0, 0, 0, 0, 0, 0, 0, 0, 0, 0,
+                         0])),
+            (38, Swap 1), (39, Arith DIV), (40, Stack (PUSH_N [255, 255, 255, 255])), (45, Bits inst_AND),
+            (46, Dup 1), (47, Stack (PUSH_N [62, 203, 94, 223])), (52, Arith inst_EQ),
+            (53, Stack (PUSH_N [71]))],
+        Jumpi),
+       (56, [(56, Dup 1), (57, Stack (PUSH_N [140, 213, 176, 119])), (62, Arith inst_EQ),
+             (63, Stack (PUSH_N [123]))],
+        Jumpi),
+       (66, [(66, Pc JUMPDEST), (67, Stack (PUSH_N [0])), (69, Dup 1), (70, Unknown 253)], Next),
+       (71, [(71, Pc JUMPDEST), (72, Info CALLVALUE), (73, Arith ISZERO), (74, Stack (PUSH_N [81]))], Jumpi),
+       (77, [(77, Stack (PUSH_N [0])), (79, Dup 1), (80, Unknown 253)], Next),
+       (81, [(81, Pc JUMPDEST), (82, Stack (PUSH_N [101])), (84, Stack (PUSH_N [4])), (86, Dup 1), (87, Dup 1),
+             (88, Stack CALLDATALOAD), (89, Swap 1), (90, Stack (PUSH_N [32])), (92, Arith ADD), (93, Swap 1),
+             (94, Swap 2), (95, Swap 1), (96, Stack POP), (97, Stack POP), (98, Stack (PUSH_N [161]))],
+        Jump),
+       (101, [(101, Pc JUMPDEST), (102, Stack (PUSH_N [64])), (104, Memory MLOAD), (105, Dup 1), (106, Dup 3),
+              (107, Dup 2), (108, Memory MSTORE), (109, Stack (PUSH_N [32])), (111, Arith ADD), (112, Swap 2),
+              (113, Stack POP), (114, Stack POP), (115, Stack (PUSH_N [64])), (117, Memory MLOAD),
+              (118, Dup 1), (119, Swap 2), (120, Arith SUB), (121, Swap 1), (122, Misc RETURN)],
+        No),
+       (123, [(123, Pc JUMPDEST), (124, Info CALLVALUE), (125, Arith ISZERO), (126, Stack (PUSH_N [133]))],
+        Jumpi),
+       (129, [(129, Stack (PUSH_N [0])), (131, Dup 1), (132, Unknown 253)], Next),
+       (133, [(133, Pc JUMPDEST), (134, Stack (PUSH_N [139])), (136, Stack (PUSH_N [173]))], Jump),
+       (139, [(139, Pc JUMPDEST), (140, Stack (PUSH_N [64])), (142, Memory MLOAD), (143, Dup 1), (144, Dup 3),
+              (145, Dup 2), (146, Memory MSTORE), (147, Stack (PUSH_N [32])), (149, Arith ADD), (150, Swap 2),
+              (151, Stack POP), (152, Stack POP), (153, Stack (PUSH_N [64])), (155, Memory MLOAD),
+              (156, Dup 1), (157, Swap 2), (158, Arith SUB), (159, Swap 1), (160, Misc RETURN)],
+        No),
+       (161, [(161, Pc JUMPDEST), (162, Stack (PUSH_N [0])), (164, Stack (PUSH_N [1])), (166, Swap 1),
+              (167, Stack POP)],
+        Next),
+       (168, [(168, Pc JUMPDEST), (169, Swap 2), (170, Swap 1), (171, Stack POP)], Jump),
+       (173, [(173, Pc JUMPDEST), (174, Stack (PUSH_N [0])), (176, Stack (PUSH_N [2])), (178, Swap 1),
+              (179, Stack POP)],
+        Next),
+       (180, [(180, Pc JUMPDEST), (181, Swap 1)], Jump), (183, [(183, Misc STOP)], No),
+       (184, [(184, Log LOG1), (185, Stack (PUSH_N [98, 122, 122, 114, 48, 88])), (192, Arith SHA3),
+              (193, Unknown 201), (194, Unknown 207), (195, Unknown 30), (196, Swap 14), (197, Dup 4),
+              (198, Stack (PUSH_N
+                            [31, 111, 154, 254, 206, 166, 43, 126, 134, 141, 152, 80, 46, 232, 85, 109, 202,
+                             246, 171])),
+              (218, Unknown 178), (219, Unknown 74), (220, Unknown 203), (221, Dup 12), (222, Unknown 192),
+              (223, Unknown 217), (224, Unknown 251), (225, Misc STOP)],
+        No),
+       (226, [(226, Unknown 41)], Next)],
+    all_blocks =
+      [(0, [(0, Stack (PUSH_N [96])), (2, Stack (PUSH_N [64])), (4, Memory MSTORE), (5, Stack (PUSH_N [0])),
+            (7, Stack CALLDATALOAD),
+            (8, Stack (PUSH_N
+                        [1, 0, 0, 0, 0, 0, 0, 0, 0, 0, 0, 0, 0, 0, 0, 0, 0, 0, 0, 0, 0, 0, 0, 0, 0, 0, 0, 0,
+                         0])),
+            (38, Swap 1), (39, Arith DIV), (40, Stack (PUSH_N [255, 255, 255, 255])), (45, Bits inst_AND),
+            (46, Dup 1), (47, Stack (PUSH_N [62, 203, 94, 223])), (52, Arith inst_EQ),
+            (53, Stack (PUSH_N [71]))],
+        Jumpi),
+       (56, [(56, Dup 1), (57, Stack (PUSH_N [140, 213, 176, 119])), (62, Arith inst_EQ),
+             (63, Stack (PUSH_N [123]))],
+        Jumpi),
+       (66, [(66, Pc JUMPDEST), (67, Stack (PUSH_N [0])), (69, Dup 1), (70, Unknown 253)], Next),
+       (71, [(71, Pc JUMPDEST), (72, Info CALLVALUE), (73, Arith ISZERO), (74, Stack (PUSH_N [81]))], Jumpi),
+       (77, [(77, Stack (PUSH_N [0])), (79, Dup 1), (80, Unknown 253)], Next),
+       (81, [(81, Pc JUMPDEST), (82, Stack (PUSH_N [101])), (84, Stack (PUSH_N [4])), (86, Dup 1), (87, Dup 1),
+             (88, Stack CALLDATALOAD), (89, Swap 1), (90, Stack (PUSH_N [32])), (92, Arith ADD), (93, Swap 1),
+             (94, Swap 2), (95, Swap 1), (96, Stack POP), (97, Stack POP), (98, Stack (PUSH_N [161]))],
+        Jump),
+       (101, [(101, Pc JUMPDEST), (102, Stack (PUSH_N [64])), (104, Memory MLOAD), (105, Dup 1), (106, Dup 3),
+              (107, Dup 2), (108, Memory MSTORE), (109, Stack (PUSH_N [32])), (111, Arith ADD), (112, Swap 2),
+              (113, Stack POP), (114, Stack POP), (115, Stack (PUSH_N [64])), (117, Memory MLOAD),
+              (118, Dup 1), (119, Swap 2), (120, Arith SUB), (121, Swap 1), (122, Misc RETURN)],
+        No),
+       (123, [(123, Pc JUMPDEST), (124, Info CALLVALUE), (125, Arith ISZERO), (126, Stack (PUSH_N [133]))],
+        Jumpi),
+       (129, [(129, Stack (PUSH_N [0])), (131, Dup 1), (132, Unknown 253)], Next),
+       (133, [(133, Pc JUMPDEST), (134, Stack (PUSH_N [139])), (136, Stack (PUSH_N [173]))], Jump),
+       (139, [(139, Pc JUMPDEST), (140, Stack (PUSH_N [64])), (142, Memory MLOAD), (143, Dup 1), (144, Dup 3),
+              (145, Dup 2), (146, Memory MSTORE), (147, Stack (PUSH_N [32])), (149, Arith ADD), (150, Swap 2),
+              (151, Stack POP), (152, Stack POP), (153, Stack (PUSH_N [64])), (155, Memory MLOAD),
+              (156, Dup 1), (157, Swap 2), (158, Arith SUB), (159, Swap 1), (160, Misc RETURN)],
+        No),
+       (161, [(161, Pc JUMPDEST), (162, Stack (PUSH_N [0])), (164, Stack (PUSH_N [1])), (166, Swap 1),
+              (167, Stack POP)],
+        Next),
+       (168, [(168, Pc JUMPDEST), (169, Swap 2), (170, Swap 1), (171, Stack POP)], Jump),
+       (173, [(173, Pc JUMPDEST), (174, Stack (PUSH_N [0])), (176, Stack (PUSH_N [2])), (178, Swap 1),
+              (179, Stack POP)],
+        Next),
+       (180, [(180, Pc JUMPDEST), (181, Swap 1)], Jump), (183, [(183, Misc STOP)], No),
+       (184, [(184, Log LOG1), (185, Stack (PUSH_N [98, 122, 122, 114, 48, 88])), (192, Arith SHA3),
+              (193, Unknown 201), (194, Unknown 207), (195, Unknown 30), (196, Swap 14), (197, Dup 4),
+              (198, Stack (PUSH_N
+                            [31, 111, 154, 254, 206, 166, 43, 126, 134, 141, 152, 80, 46, 232, 85, 109, 202,
+                             246, 171])),
+              (218, Unknown 178), (219, Unknown 74), (220, Unknown 203), (221, Dup 12), (222, Unknown 192),
+              (223, Unknown 217), (224, Unknown 251), (225, Misc STOP)],
+        No),
+       (226, [(226, Unknown 41)], Next)]\<rparr>"
+
+lemma
+"triple_blocks blocks (initial_state ** (data_lst dispatch1_hash) ** sent_value 0) (action (ContractReturn (word_rsplit (1:: w256))))"
+apply (simp add: blocks_def)
+
+sorry
+typ "256 word \<Rightarrow> (byte list \<Rightarrow> byte list)"
+lemma
+"triple_blocks blocks (initial_state ** (data_lst dispatch_hash) ** ( if dispatch_hash = dispatch1_hash then (data_lst dispatch_hash) else emp) ** sent_value 0) 
+( if dispatch_hash = dispatch1_hash then action (ContractReturn (word_rsplit (1:: w256))) else ())"
+apply (simp add: blocks_def)
+
+
+end
